coq/LambdaNRA/Typing/TLambdaNRA.v
@@ -1,0 +1,359 @@
+(*
+ * Copyright 2015-2016 IBM Corporation
+ *
+ * Licensed under the Apache License, Version 2.0 (the "License");
+ * you may not use this file except in compliance with the License.
+ * You may obtain a copy of the License at
+ *
+ * http://www.apache.org/licenses/LICENSE-2.0
+ *
+ * Unless required by applicable law or agreed to in writing, software
+ * distributed under the License is distributed on an "AS IS" BASIS,
+ * WITHOUT WARRANTIES OR CONDITIONS OF ANY KIND, either express or implied.
+ * See the License for the specific language governing permissions and
+ * limitations under the License.
+ *)
+
+Section TLambdaNRA.
+  Require Import String.
+  Require Import List.
+  Require Import Compare_dec.
+  Require Import Program.
+  Require Import EquivDec.
+  Require Import Morphisms.
+  
+  Require Import Utils BasicSystem.
+  Require Import LambdaNRA.
+
+  (** Typing for LambdaNRA *)
+  Section typ.
+    Context {m:basic_model}.
+    Context (τconstants:tbindings).
+   
+    Inductive lambda_nra_type : lambda_nra -> tbindings -> rtype -> Prop :=
+    | LTVar {Γ τ} v :
+        tdot Γ v = Some τ ->
+        lambda_nra_type (LNRAVar v) Γ τ
+    | TLTable {Γ τ} s :
+      tdot τconstants s = Some τ ->
+      lambda_nra_type (LNRATable s) Γ τ
+  | TLConst {Γ τ} c :
+      data_type (normalize_data brand_relation_brands c) τ ->
+      lambda_nra_type (LNRAConst c) Γ τ
+  | TLBinop {Γ τ₁ τ₂ τ} b op1 op2 :
+      (* b : (τ₁,τ₂) -> τout
+         op₁ : τin -> τ₁
+         op₂ : τin -> τ₂
+         ==========================
+         b (op₁,op₂) : τin -> τout *)
+      binOp_type b τ₁ τ₂ τ ->
+      lambda_nra_type op1 Γ τ₁ ->
+      lambda_nra_type op2 Γ τ₂ ->
+      lambda_nra_type (LNRABinop b op1 op2) Γ τ
+  | TLUnop {Γ τ₀ τ } u op :
+      unaryOp_type u τ₀ τ ->
+      lambda_nra_type op Γ τ₀ ->
+      lambda_nra_type (LNRAUnop u op) Γ τ
+  | TLMap {Γ τ₀ τ} lop1 op2 :
+      lnra_lambda_type lop1 Γ τ₀ τ ->
+      lambda_nra_type op2 Γ (Coll τ₀) ->
+      lambda_nra_type (LNRAMap lop1 op2) Γ (Coll τ)
+  | TLMapConcat {Γ τ₁ τ₂ τ} lop1 op2 pf1 pf2 pf3 :
+      lnra_lambda_type lop1 Γ (Rec Closed τ₁ pf1) (Coll (Rec Closed τ₂ pf2)) ->
+      lambda_nra_type op2 Γ (Coll (Rec Closed τ₁ pf1)) ->
+      rec_concat_sort τ₁ τ₂ = τ ->
+      lambda_nra_type (LNRAMapConcat lop1 op2) Γ (Coll (Rec Closed τ pf3))
+  | ATProduct {Γ τ₁ τ₂ τ} op1 op2 pf1 pf2 pf3 :
+      lambda_nra_type op1 Γ (Coll (Rec Closed τ₁ pf1)) ->
+      lambda_nra_type op2 Γ (Coll (Rec Closed τ₂ pf2)) ->
+      rec_concat_sort τ₁ τ₂ = τ ->
+      lambda_nra_type (LNRAProduct op1 op2) Γ(Coll (Rec Closed τ pf3))
+  | ATFilter {Γ τ} lop1 op2 :
+      lnra_lambda_type lop1 Γ τ Bool ->
+      lambda_nra_type op2 Γ (Coll τ) ->
+      lambda_nra_type (LNRAFilter lop1 op2) Γ (Coll τ)
+    with
+    lnra_lambda_type :  lnra_lambda -> tbindings -> rtype -> rtype -> Prop :=
+    | TLLambda {Γ τin τout} x e :
+        lambda_nra_type e (rec_sort (Γ++[(x,τin)])) τout ->
+        lnra_lambda_type (LNRALambda x e) Γ τin τout
+    .
+                                     
+  End typ.
+
+
+  (** Type lemmas for individual algebraic expressions *)
+  Context {m:basic_model}.
+
+  (** Main lemma for the type correctness of NNNRC *)
+
+  (* TODO: move this lemma *)
+  Lemma assoc_lookupr_equiv_cons_in {A B} {dec:EqDec A eq} (s:A) (d:B) l :
+    In s (domain l) -> 
+    assoc_lookupr_equiv l ((s, d) :: l).
+  Proof.
+    unfold assoc_lookupr_equiv; intros.
+    simpl.
+    match_case; intros.
+    match_case; intros.
+    unfold equiv in *; subst.
+    apply assoc_lookupr_none_nin in H0.
+    congruence.
+  Qed.
+
+    Theorem typed_lambda_nra_yields_typed_data
+          {τ}
+          (cenv:bindings)
+          (τc:tbindings)
+          (env:bindings)
+          (Γ:tbindings)
+          (e:lambda_nra) :
+    bindings_type cenv τc ->
+    bindings_type env Γ ->
+    lambda_nra_type τc e Γ τ ->
+    (exists x,
+        (lambda_nra_eval brand_relation_brands cenv env e) = Some x
+        /\ (data_type x τ)).
+    Proof.
+      intros cbt.
+      revert env Γ τ.
+      induction e; intros env Γ τ bt et
+      ; invcs et
+      ; autorewrite with lambda_nra
+      ; simpl.
+      - unfold bindings_type in *.
+      clear cbt.
+      unfold tdot, edot in *.
+      dependent induction bt; intros; try discriminate.
+      destruct x; destruct y; destruct H; simpl in *; subst.
+      match_case_in H0; [intros ? eqq | intros eqq]; rewrite eqq in H0.
+      + invcs H0; destruct (IHbt eqq) as [dd [edd tdd]].
+         rewrite edd.
+         eauto.
+      + match_destr_in H0.
+        unfold equiv in *; invcs H0.
+        apply sorted_forall_same_domain in bt.
+        apply assoc_lookupr_none_nin in eqq.
+        rewrite <- bt in eqq.
+        exists d; split; trivial.
+        match_case; intros.
+        apply assoc_lookupr_in in H.
+        apply in_dom in H.
+        congruence.
+    - unfold bindings_type in *.
+      clear bt.
+      unfold tdot, edot in *.
+      induction cbt; intros; try discriminate.
+      destruct x; destruct y; destruct H; simpl in *; subst.
+      match_case_in H0; [intros ? eqq | intros eqq]; rewrite eqq in H0.
+      + invcs H0; destruct (IHcbt eqq) as [dd [edd tdd]].
+         rewrite edd.
+         eauto.
+      + match_destr_in H0.
+        unfold equiv in *; invcs H0.
+        apply sorted_forall_same_domain in cbt.
+        apply assoc_lookupr_none_nin in eqq.
+        rewrite <- cbt in eqq.
+        exists d; split; trivial.
+        match_case; intros.
+        apply assoc_lookupr_in in H.
+        apply in_dom in H.
+        congruence.
+    - eauto. 
+    - destruct (IHe1 _ _ _ bt H5) as [dd1 [edd1 tdd1]]; 
+      destruct (IHe2 _ _ _ bt H6) as [dd2 [edd2 tdd2]].
+      rewrite edd1; rewrite edd2.
+      simpl; apply (@typed_binop_yields_typed_data _ _ _ _ _ _ _ _ τ₁ τ₂ τ); assumption.
+    - destruct (IHe _ _ _ bt H4) as [dd [edd tdd]].
+      rewrite edd.
+      simpl; apply (@typed_unop_yields_typed_data _ _ _ _ _ _ _ _ τ₀ τ); assumption.
+    - destruct (IHe2 _ _ _ bt H4) as [dd2 [edd2 tdd2]].
+      rewrite edd2; simpl.
+      dtype_inverter.
+      invcs H1.
+      invcs tdd2; rtype_equalizer; subst.
+      clear edd2.
+      induction dd2; simpl.
+      + eexists; split; [reflexivity|]. repeat constructor.
+      + invcs H1.
+        destruct (IHdd2 H3) as [dd1 [edd1 tdd1]].
+        apply some_lift in edd1.
+        destruct edd1 as [dd11 ? tdd11]; subst.
+        rewrite e.
+        rewrite lnra_lambda_eval_lambda_eq.
+        assert (bt1:bindings_type (rec_sort (env ++ [(s, a)])) (rec_sort (Γ ++ [(s, τ₀)])) ).
+        {
+          apply bindings_type_sort.
+          unfold bindings_type.
+          apply Forall2_app; trivial.
+          constructor; simpl; intuition. 
+        }
+        destruct (IHe1 _ _ _ bt1 H6) as [dd3 [edd3 tdd3]].
+        rewrite edd3.
+        simpl.
+        eexists; split; [reflexivity | ].
+        invcs tdd1; rtype_equalizer; subst.
+        constructor; constructor; trivial.
+    - destruct (IHe2 _ _ _ bt H2) as [dd2 [edd2 tdd2]].
+      rewrite edd2; simpl.
+      dtype_inverter.
+      invcs H1.
+      apply Col_inv in tdd2.
+      clear edd2.
+      induction dd2; simpl.
+      + eexists; split; [reflexivity|]. repeat constructor.
+      + invcs tdd2.
+        destruct (IHdd2 H3) as [dd1 [edd1 tdd1]].
+        apply some_lift in edd1.
+        destruct edd1 as [dd11 ? tdd11]; subst.
+        assert (bt1:bindings_type (rec_sort (env ++ [(s, a)])) (rec_sort (Γ ++ [(s, Rec Closed τ₁ pf1)])) ).
+        {
+          apply bindings_type_sort.
+          unfold bindings_type.
+          apply Forall2_app; trivial.
+          constructor; simpl; intuition. 
+        }
+        destruct (IHe1 _ _ _ bt1 H6) as [dd3 [edd3 tdd3]].
+        rewrite (rmap_concat_ext _  (fun d => lambda_nra_eval brand_relation_brands cenv (rec_sort (env ++ [(s, d)])) e1));
+          [ | intros; apply lnra_lambda_eval_lambda_eq ].
+        dtype_inverter.
+        apply Col_inv in tdd3.
+        apply Col_inv in tdd1.
+        assert (part1pf:exists part1, oomap_concat (fun d => lambda_nra_eval brand_relation_brands cenv 
+                                                                             (rec_sort (env ++ [(s, d)])) e1) (drec a) = Some part1 /\ Forall (fun d : data => d ▹ Rec Closed (rec_concat_sort τ₁ τ₂) pf3) part1
+).
+        {
+          unfold oomap_concat.
+          rewrite edd3.
+          unfold omap_concat.
+          clear edd3.
+          revert dd3 tdd3 H1; clear; intros.
+          induction dd3.
+          - eexists; split; [reflexivity | ]; constructor.
+          - invcs tdd3.
+            dtype_inverter.
+            destruct (IHdd3 H3) as [part1 [part1eq part1t]].
+            unfold orecconcat in part1eq.
+            rewrite part1eq.
+            simpl.
+            eexists; split; [reflexivity | ].
+            constructor; trivial.
+            apply dtrec_closed_inv in H1.
+            apply dtrec_closed_inv in H2.
+            apply dtrec_full.
+            apply rec_concat_with_drec_concat_well_typed; auto.
+        }
+        destruct part1pf as [part1 [part1eq part1t]].
+        erewrite rmap_concat_cons; eauto.
+        simpl; eexists; split; [reflexivity | ].
+        constructor.
+        apply Forall_app; trivial.
+    - destruct (IHe1 _ _ _ bt H1) as [dd1 [edd1 tdd1]]; 
+      destruct (IHe2 _ _ _ bt H2) as [dd2 [edd2 tdd2]].
+      rewrite edd1; rewrite edd2.
+      clear edd1 edd2.
+      dtype_inverter.
+      apply Col_inv in tdd1.
+      apply Col_inv in tdd2.
+      clear IHe1 IHe2 cbt bt.
+      induction dd1; simpl.
+      + eexists; split; [reflexivity | ]; repeat constructor.
+      + invcs tdd1.
+        destruct (IHdd1 H4) as [dd3 [dde3 ddt3]]; clear IHdd1.
+        apply some_lift in dde3.
+        destruct dde3 as [dd33 dde33 ?]; subst.
+        assert (part1pf:exists part1, oomap_concat (fun _ : data => Some (dcoll dd2)) a = Some part1 /\ Forall (fun d : data => d ▹ Rec Closed (rec_concat_sort τ₁ τ₂) pf3) part1).
+        {
+          clear  dd33 dde33 ddt3.
+          unfold oomap_concat.
+          dtype_inverter.
+          apply dtrec_closed_inv in H3.
+          unfold omap_concat.
+          unfold orecconcat.
+          induction dd2; simpl.
+          - eexists; split; [reflexivity | ]; constructor.
+          - invcs tdd2.
+            destruct (IHdd2 H6) as [part1 [part1e part1t]].
+            rewrite part1e; clear part1e.
+            dtype_inverter.
+            eexists; split; [reflexivity | ].
+            constructor; trivial.
+            apply dtrec_full.
+            apply dtrec_closed_inv in H5.
+            apply rec_sort_Forall2.
+            + repeat rewrite domain_app; f_equal;
+              eapply sorted_forall_same_domain; eauto.
+            + apply Forall2_app; trivial.
+        } 
+        dtype_inverter.
+        apply Col_inv in ddt3.
+        destruct part1pf as [part1 [part1eq part1t]].
+        erewrite rmap_concat_cons; eauto.
+        simpl; eexists; split; [reflexivity | ].
+        constructor.
+        apply Forall_app; trivial.
+    - destruct (IHe2 _ _ _ bt H4) as [dd2 [edd2 tdd2]].
+      rewrite edd2; simpl; clear edd2 H4.
+      dtype_inverter.
+      invcs H1.
+      apply Col_inv in tdd2.
+      induction dd2; simpl.
+      + eexists; split; [reflexivity|]. repeat constructor.
+      + invcs tdd2.
+        destruct (IHdd2 H2) as [dd1 [edd1 tdd1]].
+        apply some_lift in edd1.
+        destruct edd1 as [dd11 dd11e dd11t]; subst.
+        rewrite dd11e.
+        rewrite lnra_lambda_eval_lambda_eq.
+        assert (bt1:bindings_type (rec_sort (env ++ [(s, a)])) (rec_sort (Γ ++ [(s, τ0)])) ).
+        {
+          apply bindings_type_sort.
+          unfold bindings_type.
+          apply Forall2_app; trivial.
+          constructor; simpl; intuition. 
+        }
+        destruct (IHe1 _ _ _ bt1 H5) as [dd3 [edd3 tdd3]].
+        rewrite edd3.
+        dtype_inverter.
+        apply Col_inv in tdd1.
+        destruct x; simpl; (eexists; split; [reflexivity | ]).
+        * constructor; constructor; trivial.
+        * constructor; trivial.
+    Qed.
+
+    (* we are only sensitive to the environment up to lookup *)
+  Global Instance nnrc_type_lookup_equiv_prop {m:basic_model} :
+    Proper (assoc_lookupr_equiv ==> eq ==> assoc_lookupr_equiv ==> eq ==> iff) lambda_nra_type.
+  Proof.
+    cut (Proper (assoc_lookupr_equiv ==> eq ==> assoc_lookupr_equiv ==> eq ==> impl) lambda_nra_type);
+    unfold Proper, respectful, iff, impl; intros; subst;
+      [unfold assoc_lookupr_equiv in *; intuition; eauto | ].
+    rename y0 into e.
+    rename x into cenv1.
+    rename y into cenv2.
+    rename x1 into env1.
+    rename y1 into env2.
+    rename y2 into τ.
+    rename H into ceqs.
+    rename H1 into eqs.
+    rename H3 into et.
+    revert env1 env2 τ eqs et.
+    induction e; simpl; inversion 2; subst; econstructor; eauto 3
+    ; try solve [
+            constructor
+            ; invcs H1
+            ; eapply IHe1; [ | eassumption]
+            ; rewrite eqs; reflexivity].
+    - unfold tdot, edot in *; unfold assoc_lookupr_equiv in *; simpl in *.
+      rewrite <- eqs; trivial.
+    - unfold tdot, edot in *; unfold assoc_lookupr_equiv in *; simpl in *.
+      rewrite <- ceqs; trivial.
+  Qed.
+  
+End TLambdaNRA.
+
+(* 
+*** Local Variables: ***
+*** coq-load-path: (("../../../coq" "Qcert")) ***
+*** End: ***
+*)
